feat: 1 2 4 finish

qcp/ast/annotated_C/ast.h
@@ -16,13 +16,14 @@
 /*@ Extern Coq (const_type :: *)*/
 /*@ Extern Coq (quant_type :: *)*/
 /*@ Extern Coq (term_type :: *)*/
-/*@ Extern Coq (store_string : Z -> list Z -> Assertion)
+/*@ Extern Coq (CImpl : const_type) 
+               (store_string : Z -> list Z -> Assertion)
                (store_term : Z -> term -> Assertion)
                (store_term' : Z -> term -> Assertion)
                (store_term_res : Z -> option term -> Assertion)
                (store_term_cell : Z -> term -> Assertion)
                (sll_term_list : Z -> list term -> Assertion)
-               (sllseg_term_list : Z -> list term -> Assertion)
+               (sllseg_term_list : Z -> Z -> list term -> Assertion)
                (sllbseg_term_list : Z -> Z -> list term -> Assertion)
                (store_partial_quant : Z -> Z -> partial_quant -> Assertion)
                (store_var_sub : Z -> var_sub -> Assertion)
@@ -34,6 +35,7 @@
                (store_solve_res' : Z -> solve_res -> Assertion)
                (store_ImplyProp : Z -> Z -> Z -> term -> term -> Assertion)
                (store_imply_res : Z -> option ImplyProp -> Assertion)
+               (store_sep_imp_res : Z -> Z -> term -> Assertion)
                (list_Z_cmp : list Z -> list Z -> Z)
                (term_alpha_eqn : term -> term -> Z)
                (term_subst_v : list Z -> list Z -> term -> term)
@@ -160,11 +162,8 @@ ImplyProp *createImplyProp(term *t1, term *t2)
     /*@ With term1 term2
           Require store_term(t1, term1) *
                   store_term(t2, term2)
-          Ensure exists t1' t2',
-                t1 == t1@pre && t2 == t2@pre &&
-                  store_term(t1, term1) *
-                  store_term(t2, term2) *
-                store_ImplyProp(__return, t1', t2', term1, term2)
+          Ensure  t1 == t1@pre && t2 == t2@pre &&
+                  store_ImplyProp(__return, t1, t2, term1, term2)
     */
     ;
 
