qcp/ast/VC/thm_apply_proof_manual.v
@@ -21,7 +21,6 @@ From SimpleC.EE Require Import malloc.
 From SimpleC.EE Require Import sll_tmpl.
 Local Open Scope sac.
 
-
 Lemma proof_of_sub_thm_return_wit_1 : sub_thm_return_wit_1.
 Proof.
   pre_process.
@@ -126,123 +125,123 @@ Qed.
 Lemma proof_of_separate_imply_return_wit_1 : separate_imply_return_wit_1.
 Proof.
   pre_process.
-  unfold store_imply_res.
-  unfold sep_impl.
-  destruct trm; unfold NULL in *.
-  - sep_apply (store_term_fold_out t_pre (TermVar var)).
+  unfold store_sep_imp_res.
+  destruct trm; try (unfold termtypeID in *); try congruence.
+  + unfold store_term, store_term'.
+    Intros y; Exists y; entailer!.
+  + unfold store_term, store_term'.
     entailer!.
+  + unfold store_term, store_term'.
+    fold store_term; Intros y z; Exists y z.
     entailer!.
-    lia.
-  - sep_apply store_term_fold_out.
-    entailer!.
-    entailer!.
-    lia.
-  - contradiction.
-  - sep_apply store_term_fold_out.
-    entailer!.
-    entailer!.
-    lia.
-Qed.
+Qed. 
 
 Lemma proof_of_separate_imply_return_wit_2 : separate_imply_return_wit_2.
 Proof.
   pre_process.
+  unfold store_sep_imp_res.
   rewrite H1.
-  unfold store_term at 2.
-  fold store_term.
-  Exists v_2 v.
-  entailer!.
-  sep_apply store_term_fold_out.
-  entailer!.
-
-  unfold store_imply_res.
-  unfold sep_impl.
-  destruct lt.
-
-  - entailer!.
-  - entailer!.
-  - contradiction.
-  - entailer!.
-  - lia.
+  destruct lt; try (unfold termtypeID in *); try congruence.
+  + unfold store_term, store_term'.
+    fold store_term.
+    unfold termtypeID.
+    Intros y; Exists v_2 v y. entailer!.
+  + unfold store_term, store_term'.
+    fold store_term.
+    Exists v_2 v; entailer!.
+  + unfold store_term, store_term'.
+    unfold termtypeID.
+    fold store_term; Intros y z; Exists v_2 v y z.
+    entailer!.
 Qed.
 
 Lemma proof_of_separate_imply_return_wit_3 : separate_imply_return_wit_3.
 Proof.
   pre_process.
-  rewrite H4.
-  unfold store_term at 3.
-  fold store_term.
-  rewrite H1.
-  unfold store_term at 3.
-  fold store_term.
-  Exists v_2 v v_4 v_3.
-
-  sep_apply ((store_term_fold_out v_4 ll) H0).
-  entailer!.
-
-  unfold store_imply_res.
-  unfold sep_impl.
-  destruct ll.
-  - entailer!.
-  - contradiction.
-  - entailer!.
-  - entailer!.
+  unfold store_sep_imp_res.
+  rewrite H4, H1.
+  destruct ll; try (unfold termtypeID in *); try congruence.
+  + unfold store_term, store_term'.
+    fold store_term.
+    Intros yyy.
+    Exists v_2 v.
+    Exists v_4 v_3.
+    Exists yyy.
+    unfold termtypeID.
+    entailer!.
+  + unfold store_term, store_term'.
+    fold store_term.
+    Intros yyy zzz.
+    Exists v_2 v.
+    Exists v_4 v_3.
+    Exists yyy zzz.
+    unfold termtypeID.
+    entailer!.
+  + unfold store_term, store_term'.
+    fold store_term.
+    Intros yyy zzz.
+    Exists v_2 v.
+    Exists v_4 v_3.
+    Exists yyy zzz.
+    unfold termtypeID.
+    entailer!.
 Qed.
 
 Lemma proof_of_separate_imply_return_wit_4 : separate_imply_return_wit_4.
 Proof.
   pre_process.
-  rewrite H6.
-  unfold store_term at 3.
-  fold store_term.
-  Exists v_2 v.
-  entailer!.
-
-  rewrite H3.
-  unfold store_term at 2.
-  fold store_term.
-  Exists v_4 v_3.
-  entailer!.
-
-  rewrite H0.
-  unfold store_term.
-  entailer!.
-
-  unfold store_imply_res.
-  unfold sep_impl.
-  destruct llctype.
-  - entailer!.
-  - entailer!.
-  - entailer!.
-  - entailer!.
-  - entailer!.
-  - entailer!.
-  - entailer!.
-  - contradiction.
-Qed. 
-
-Lemma proof_of_separate_imply_return_wit_5 : separate_imply_return_wit_5.
-Proof.
-  pre_process.
-  unfold store_imply_res.
-  unfold sep_impl.
-  rewrite H6.
-  rewrite H3.
-  rewrite H0.
-  destruct llctype.
-  - unfold ctID in H; lia.
-  - unfold ctID in H; lia.
-  - unfold ctID in H; lia.
-  - unfold ctID in H; lia.
-  - unfold ctID in H; lia.
-  - unfold ctID in H; lia.
-  - unfold ctID in H; lia.
-  - Exists t1' t2'.
-    unfold store_term.
+  unfold store_sep_imp_res.
+  rewrite H6, H3, H0.
+  unfold ctID in H.
+  destruct llctype; try congruence.
+  + unfold store_term, store_term'.
     fold store_term.
     Exists v_2 v.
     Exists v_4 v_3.
     entailer!.
+  + unfold store_term, store_term'.
+    fold store_term.
+    Exists v_2 v.
+    Exists v_4 v_3.
+    entailer!.
+  + unfold store_term, store_term'.
+    fold store_term.
+    Exists v_2 v.
+    Exists v_4 v_3.
+    entailer!.
+  + unfold store_term, store_term'.
+    fold store_term.
+    Exists v_2 v.
+    Exists v_4 v_3.
+    entailer!.
+  + unfold store_term, store_term'.
+    fold store_term.
+    Exists v_2 v.
+    Exists v_4 v_3.
+    entailer!.
+  + unfold store_term, store_term'.
+    fold store_term.
+    Exists v_2 v.
+    Exists v_4 v_3.
+    entailer!.
+  + unfold store_term, store_term'.
+    fold store_term.
+    Exists v_2 v.
+    Exists v_4 v_3.
+    entailer!.
+Qed.
+
+Lemma proof_of_separate_imply_return_wit_5 : separate_imply_return_wit_5.
+Proof. 
+  pre_process.
+  unfold store_sep_imp_res.
+  rewrite H6, H3, H0.
+  unfold ctID in H.
+  destruct llctype; try congruence.
+  unfold termtypeID.
+  Exists v_2 v.
+  Exists v_4 v_3.
+  entailer!.
 Qed.
 
 Lemma proof_of_separate_imply_which_implies_wit_1 : separate_imply_which_implies_wit_1.
@@ -304,6 +303,36 @@ Proof.
   lia.
   lia.
 Qed. 
+
+Lemma proof_of_check_list_gen_entail_wit_2 : check_list_gen_entail_wit_2.
+Proof. Admitted. 
+
+Lemma proof_of_check_list_gen_return_wit_1 : check_list_gen_return_wit_1.
+Proof. Admitted. 
+
+Lemma proof_of_check_list_gen_return_wit_2_1 : check_list_gen_return_wit_2_1.
+Proof. Admitted. 
+
+Lemma proof_of_check_list_gen_return_wit_2_2 : check_list_gen_return_wit_2_2.
+Proof. Admitted. 
+
+Lemma proof_of_check_list_gen_return_wit_3 : check_list_gen_return_wit_3.
+Proof. Admitted. 
+
+Lemma proof_of_check_list_gen_which_implies_wit_1 : check_list_gen_which_implies_wit_1.
+Proof. Admitted. 
+
+Lemma proof_of_check_list_gen_which_implies_wit_2 : check_list_gen_which_implies_wit_2.
+Proof. Admitted. 
+
+Lemma proof_of_check_list_gen_which_implies_wit_3 : check_list_gen_which_implies_wit_3.
+Proof. Admitted. 
+
+Lemma proof_of_check_list_gen_which_implies_wit_4 : check_list_gen_which_implies_wit_4.
+Proof. Admitted. 
+
+Lemma proof_of_check_list_gen_which_implies_wit_5 : check_list_gen_which_implies_wit_5.
+Proof. Admitted. 
 
 Lemma proof_of_thm_apply_return_wit_1_1 : thm_apply_return_wit_1_1.
 Proof.
@@ -380,3 +409,4 @@ Proof.
   Exists 0; rewrite H.
   entailer!.
 Admitted.
+
